Make term_meta definitions opaque.

cryptis.v
@@ -897,26 +897,36 @@ rewrite lookup_op !lookup_singleton -Some_op Some_valid.
 by move=> /to_agree_op_inv_L ->.
 Qed.
 
-Definition term_token t E : iProp :=
+Definition term_token_def t E : iProp :=
   ∃ γ, term_name t γ ∗ gmeta_token γ E.
+Definition term_token_aux : seal term_token_def. by eexists. Qed.
+Definition term_token := unseal term_token_aux.
+Lemma term_token_unseal : term_token = term_token_def.
+Proof. exact: seal_eq. Qed.
 
-Definition term_meta `{Countable L} t N (x : L) : iProp :=
+Definition term_meta_def `{Countable L} t N (x : L) : iProp :=
   ∃ γ, term_name t γ ∗ gmeta γ N x.
+Definition term_meta_aux : seal (@term_meta_def). by eexists. Qed.
+Definition term_meta := unseal term_meta_aux.
+Lemma term_meta_unseal : @term_meta = @term_meta_def.
+Proof. exact: seal_eq. Qed.
+Arguments term_meta {L _ _} t N x.
 
 Global Instance term_token_timeless t E : Timeless (term_token t E).
-Proof. apply _. Qed.
+Proof. rewrite term_token_unseal. apply _. Qed.
 
 Global Instance term_meta_timeless `{Countable L} t N (x : L) :
   Timeless (term_meta t N x).
-Proof. apply _. Qed.
+Proof. rewrite term_meta_unseal. apply _. Qed.
 
 Global Instance term_meta_persistent `{Countable L} t N (x : L) :
   Persistent (term_meta t N x).
-Proof. apply _. Qed.
+Proof. rewrite term_meta_unseal. apply _. Qed.
 
 Lemma term_token_drop E1 E2 t :
   E1 ⊆ E2 → term_token t E2 -∗ term_token t E1.
 Proof.
+rewrite term_token_unseal.
 iIntros "% (%γ & #name & token)".
 iExists γ. iSplit => //. by iApply gmeta_token_drop.
 Qed.
@@ -924,6 +934,7 @@ Qed.
 Lemma term_token_disj E1 E2 t :
   term_token t E1 -∗ term_token t E2 -∗ ⌜E1 ## E2⌝.
 Proof.
+rewrite term_token_unseal.
 iIntros "(% & #name1 & token1) (% & #name2 & token2)".
 iPoseProof (term_name_agree with "name1 name2") as "<-".
 iApply (gmeta_token_disj with "token1 token2").
@@ -932,6 +943,7 @@ Qed.
 Lemma term_token_difference t E1 E2 :
   E1 ⊆ E2 → term_token t E2 ⊣⊢ term_token t E1 ∗ term_token t (E2 ∖ E1).
 Proof.
+rewrite term_token_unseal.
 move=> sub. iSplit.
 - iIntros "(% & #name & token)".
   rewrite (gmeta_token_difference _ _ _ sub).
@@ -946,7 +958,7 @@ Qed.
 Lemma term_meta_token `{Countable L} t (x : L) N E :
   ↑N ⊆ E → term_token t E -∗ term_meta t N x -∗ False.
 Proof.
-move=> sub.
+rewrite term_token_unseal term_meta_unseal => sub.
 iIntros "(% & #name1 & token) (% & #name2 & #meta)".
 iPoseProof (term_name_agree with "name1 name2") as "<-".
 by iApply (gmeta_gmeta_token with "token meta").
@@ -955,6 +967,7 @@ Qed.
 Lemma term_meta_set' `{Countable L} N (x : L) E t :
   ↑N ⊆ E → term_token t E ==∗ term_meta t N x ∗ term_token t (E ∖ ↑N).
 Proof.
+rewrite term_token_unseal term_meta_unseal.
 iIntros "%sub (%γ & #name & token)".
 iMod (gmeta_set' _ _ _ x sub with "token") as "[#meta token]".
 iModIntro.
@@ -972,6 +985,7 @@ Qed.
 Lemma term_meta_agree `{Countable L} t N (x1 x2 : L) :
   term_meta t N x1 -∗ term_meta t N x2 -∗ ⌜x1 = x2⌝.
 Proof.
+rewrite term_meta_unseal.
 iIntros "(% & #name1 & #meta1) (% & #name2 & #meta2)".
 iPoseProof (term_name_agree with "name1 name2") as "<-".
 iApply (gmeta_agree with "meta1 meta2").
@@ -988,14 +1002,20 @@ Qed.
 
 Section TermOwn.
 
-Context `{inG Σ A}.
-
-Definition term_own t N (x : A) : iProp :=
+Definition term_own_def `{inG Σ A} t N (x : A) : iProp :=
   ∃ γ, term_name t γ ∗ nown γ N x.
+Definition term_own_aux : seal (@term_own_def). by eexists. Qed.
+Definition term_own := unseal (@term_own_aux).
+Lemma term_own_unseal : @term_own = @term_own_def.
+Proof. exact: seal_eq. Qed.
+Arguments term_own {A _} t N x.
+
+Context `{inG Σ A}.
 
 Lemma term_own_alloc t N {E} (a : A) :
   ↑N ⊆ E → ✓ a → term_token t E ==∗ term_own t N a ∗ term_token t (E ∖ ↑N).
 Proof.
+rewrite term_own_unseal term_token_unseal.
 iIntros "%sub %val (% & #name & token)".
 iMod (nown_alloc _ _ sub val with "token") as "[own token]".
 iModIntro.
@@ -1004,12 +1024,14 @@ Qed.
 
 Lemma term_own_valid t N (a : A) : term_own t N a -∗ ✓ a.
 Proof.
+rewrite term_own_unseal.
 iIntros "(%γ' & #own_γ & own)". iApply (nown_valid with "own").
 Qed.
 
 Lemma term_own_valid_2 t N (a1 a2 : A) :
   term_own t N a1 -∗ term_own t N a2 -∗ ✓ (a1 ⋅ a2).
 Proof.
+rewrite term_own_unseal.
 iIntros "(%γ1 & #own_γ1 & own1) (%γ2 & #own_γ2 & own2)".
 iPoseProof (term_name_agree with "own_γ1 own_γ2") as "<-".
 by iApply (nown_valid_2 with "own1 own2").
@@ -1018,6 +1040,7 @@ Qed.
 Lemma term_own_update t N (a a' : A) :
   a ~~> a' → term_own t N a ==∗ term_own t N a'.
 Proof.
+rewrite term_own_unseal.
 iIntros (?) "(%γ' & #? & own)".
 iMod (nown_update with "own") as "own"; eauto.
 iModIntro. iExists γ'. eauto.
@@ -1026,24 +1049,25 @@ Qed.
 #[global]
 Instance term_own_core_persistent t N (a : A) :
   CoreId a → Persistent (term_own t N a).
-Proof. apply _. Qed.
+Proof. rewrite term_own_unseal. apply _. Qed.
 
 #[global]
 Instance term_own_timeless t N (a : A) :
   Discrete a → Timeless (term_own t N a).
-Proof. apply _. Qed.
+Proof. rewrite term_own_unseal. apply _. Qed.
 
 #[global]
-Instance term_own_ne t N : NonExpansive (term_own t N).
-Proof. solve_proper. Qed.
+Instance term_own_ne t N : NonExpansive (@term_own A _ t N).
+Proof. rewrite term_own_unseal. solve_proper. Qed.
 
 #[global]
-Instance term_own_proper t N : Proper ((≡) ==> (≡)) (term_own t N).
-Proof. solve_proper. Qed.
+Instance term_own_proper t N : Proper ((≡) ==> (≡)) (@term_own A _ t N).
+Proof. rewrite term_own_unseal. solve_proper. Qed.
 
 Lemma term_own_op t N (a1 a2 : A) :
   term_own t N (a1 ⋅ a2) ⊣⊢ term_own t N a1 ∗ term_own t N a2.
 Proof.
+rewrite term_own_unseal.
 iSplit.
 - iIntros "(%γ' & #? & [own1 own2])".
   by iSplitL "own1"; iExists γ'; iSplit.
@@ -1120,7 +1144,8 @@ assert (∀ names : gmap term gname,
     iModIntro. iExists names'. iFrame.
     rewrite dom_names' dom_insert_L. iSplit; first by iPureIntro; set_solver.
     rewrite big_sepS_union; last by set_solver.
-    iFrame. rewrite big_sepS_singleton. iExists γ. iFrame. }
+    iFrame. rewrite big_sepS_singleton.
+    rewrite term_token_unseal. iExists γ. iFrame. }
 iIntros "PE QE PQ (%names & own & #minted_names)".
 iAssert (⌜dom names ## T⌝)%I as "%dis".
 { rewrite elem_of_disjoint. iIntros "%t %t_names %t_T".
@@ -1856,10 +1881,14 @@ Arguments cryptis_key_name {Σ _}.
 Arguments key_pred {Σ _} N φ.
 Arguments key_pred_set {Σ _ _} N P.
 Arguments key_pred_token_difference {Σ _} E1 E2.
+Arguments term_token {Σ _} t E.
+Arguments term_meta {Σ _ L _ _} t N x.
 Arguments term_meta_set {Σ _ _ _ _} N x E t.
 Arguments term_token_difference {Σ _} t E1 E2.
 Arguments term_name {Σ _} t γ.
+Arguments term_own {Σ _ A _} t N x.
 Arguments term_own_alloc {Σ _ A _ t} N {_} a.
+Arguments term_own_update {Σ _ A _ t N a} a'.
 Arguments phase_inv {Σ _ _}.
 Arguments cryptis_ctx {Σ _ _}.
 Arguments unknown_alloc {Σ _}.
